---
title: Lambda Calculus
headerImg: sea.jpg
---

## Your Favorite Language

Probably has lots of features:

* Assignment (`x = x + 1`)
* Booleans, integers, characters, strings, ...
* Conditionals
* Loops
* `return`, `break`, `continue`
* Functions
* Recursion
* References / pointers
* Objects and classes
* Inheritance
* ...

Which ones can we do without?

What is the **smallest universal language**?

<br>
<br>
<br>
<br>
<br>
<br>
<br>
<br>
<br>
<br>
<br>
<br>
<br>
<br>
<br>
<br>
<br>

## What is computable?

### Before 1930s

Informal notion of an **effectively calculable** function:

![can be computed by a human with pen and paper, following an algorithm](https://oercommons.s3.amazonaws.com/media/courseware/assets/G06/06-math-math-06-9780328761197-math-9780328761197-ah-studio-images-ip3-mth-6-2-8-2-1_mw-4x3_dividehandwritten-ip3.png){#fig:pen-and-paper .align-center width=40%}


<br>
<br>
<br>
<br>

### 1936: Formalization

What is the **smallest universal language**?

![Alan Turing](https://upload.wikimedia.org/wikipedia/commons/a/a1/Alan_Turing_Aged_16.jpg){#fig:turing .align-center width=40%}

(I) final

    The [**Turing Machine**](https://en.wikipedia.org/wiki/Turing_machine)
    
<br>
<br>    
 
![Alonzo Church](https://upload.wikimedia.org/wikipedia/en/a/a6/Alonzo_Church.jpg){#fig:church .align-center width=40%}

(I) final

    The **Lambda Calculus**

<br>
<br>
<br>
<br>
<br>
<br>
<br>
<br>
<br>
<br>
<br>
<br>
<br>

## The Next 700 Languages

![Peter Landin](https://upload.wikimedia.org/wikipedia/en/f/f9/Peter_Landin.png){#fig:landin .align-center width=40%}

> Whatever the next 700 languages
> turn out to be,
> they will surely be
> variants of lambda calculus.

Peter Landin, 1966


<br>
<br>
<br>
<br>
<br>
<br>
<br>
<br>
<br>
<br>
<br>
<br>
<br>
<br>

## The Lambda Calculus

Has one feature:

* Functions

<br>
<br>
<br>
<br>
<br>
<br>
<br>
<br>
<br>
<br>

No, *really*

* ~~Assignment (`x = x + 1`)~~
* ~~Booleans, integers, characters, strings, ...~~
* ~~Conditionals~~
* ~~Loops~~
* ~~`return`, `break`, `continue`~~
* Functions
* ~~Recursion~~
* ~~References / pointers~~
* ~~Objects and classes~~
* ~~Inheritance~~
* ~~Reflection~~

<br>
<br>
<br>
<br>
<br>
<br>
<br>
<br>
<br>
<br>

More precisely, *only thing* you can do is:

* **Define** a function
* **Call** a function

<br>
<br>
<br>
<br>
<br>
<br>
<br>
<br>
<br>
<br>

## Describing a Programming Language

* _Syntax:_ what do programs look like?
* _Semantics:_ what do programs mean?
    * _Operational semantics_: how do programs execute step-by-step?

<br>
<br>
<br>
<br>
<br>
<br>
<br>
<br>
<br>
<br>

## Syntax: What Programs _Look Like_

<br>

```haskell
e ::= x
    | \x -> e
    | e1 e2
```

<br>

Programs are **expressions** `e` (also called **$\lambda$-terms**)
of one of three kinds:

- **Variable**
    - `x`, `y`, `z`
- **Abstraction** (aka _nameless_ function definition)
    - `\x -> e`
    - `x` is the _formal_ parameter, `e` is the _body_ 
    - "for any `x` compute `e`"
- **Application** (aka function call)
    - `e1 e2`
    - `e1` is the _function_, `e2` is the _argument_
    - in your favorite language: `e1(e2)`

(Here each of `e`, `e1`, `e2` can itself be a variable, abstraction, or application)

<br>
<br>
<br>
<br>
<br>
<br>
<br>
<br>
<br>
<br>

## Examples

```haskell
\x -> x             -- The identity function
                    -- ("for any x compute x")

\x -> (\y -> y)     -- A function that returns the identity function
 
\f -> f (\x -> x)   -- A function that applies its argument 
                    -- to the identity function
```

<br>
<br>
<br>
<br>
<br>
<br>
<br>
<br>
<br>
<br>
<br>
<br>


## QUIZ

Which of the following terms are syntactically **incorrect**?

**A.**  `\(\x -> x) -> y`

**B.**  `\x -> x x`

**C.**  `\x -> x (y x)`

**D.**  A and C

**E.**  all of the above

<br>

(I) final

    _Correct answer:_ **A**



<br>
<br>
<br>
<br>
<br>
<br>
<br>
<br>
<br>
<br>

## Examples

```haskell
\x -> x             -- The identity function
                    -- ("for any x compute x")

\x -> (\y -> y)     -- A function that returns the identity function
 
\f -> f (\x -> x)   -- A function that applies its argument 
                    -- to the identity function
```

<br>

How do I define a function with two arguments?

* e.g. a function that takes `x` and `y` and returns `y`?

<br>
<br>
<br>
<br>
<br>
<br>
<br>
<br>
<br>
<br>
<br>
<br>

```haskell
\x -> (\y -> y)     -- A function that returns the identity function
                    -- OR: a function that takes two arguments
                    -- and returns the second one!
```

<br>
<br>
<br>
<br>
<br>
<br>
<br>
<br>
<br>
<br>
<br>
<br>

How do I apply a function to two arguments?

* e.g. apply `\x -> (\y -> y)` to `apple` and `banana`?

<br>
<br>
<br>
<br>
<br>
<br>
<br>
<br>
<br>
<br>
<br>
<br>

```haskell
(((\x -> (\y -> y)) apple) banana) -- first apply to apple,
                                   -- then apply the result to banana
```


<br>
<br>
<br>
<br>
<br>
<br>
<br>
<br>
<br>
<br>
<br>




## Syntactic Sugar

<br>
<br>

instead of                |  we write
:-------------------------|:-------------------------
`\x -> (\y -> (\z -> e))` | `\x -> \y -> \z -> e`
`\x -> \y -> \z -> e`     | `\x y z -> e`
`(((e1 e2) e3) e4)`       |  `e1 e2 e3 e4`

<br>
<br>

```haskell
\x y -> y     -- A function that that takes two arguments
              -- and returns the second one...
              
(\x y -> y) apple banana -- ... applied to two arguments
```

<br>
<br>
<br>
<br>
<br>
<br>
<br>
<br>
<br>
<br>
<br>
<br>

## Semantics : What Programs _Mean_

<br>

How do I "run" / "execute" a $\lambda$-term?

<br>

Think of middle-school algebra:

```haskell
-- Simplify expression:

  (x + 2)*(3*x - 1)
 =
  ???
```

<br>

**Execute** = rewrite step-by-step following simple rules,
until no more rules apply

<br>
<br>
<br>
<br>
<br>
<br>
<br>
<br>
<br>
<br>
<br>
<br>

## Rewrite Rules of Lambda Calculus

<br>

1. $\alpha$-step  (aka _renaming formals_)
2. $\beta$-step   (aka _function call_)

<br>

But first we have to talk about **scope**

<br>
<br>
<br>
<br>
<br>
<br>

## Semantics: Scope of a Variable

The part of a program where a **variable is visible**

In the expression `\x -> e`

- `x` is the newly introduced variable

- `e` is **the scope** of `x`

- any occurrence of `x` in `\x -> e` is **bound** (by the **binder** `\x`)

<br>

For example, `x` is bound in:

```
  \x -> x
  \x -> (\y -> x)
```

<br>
<br>

An occurrence of `x` in `e` is **free** if it's _not bound_ by an enclosing abstraction

<br>
For example, `x` is free in:

```
  x y                -- no binders at all!  
  \y -> x y          -- no \x binder
  (\x -> \y -> y) x  -- x is outside the scope of the \x binder;
                     -- intuition: it's not "the same" x
```



<br>
<br>
<br>
<br>
<br>
<br>
<br>
<br>
<br>
<br>
<br>

## QUIZ

In the expression `(\x -> x) x`,
is `x` _bound_ or _free_?

**A.**  bound

**B.**  free

**C.**  first occurrence is bound, second is free

**D.**  first occurrence is bound, second and third are free

**E.**  first two occurrences are bound, third is free

<br>

(I) final
    
    _Correct answer:_ **C**

<br>
<br>
<br>
<br>
<br>
<br>
<br>
<br>
<br>
<br>
<br>


## Free Variables

An variable `x` is **free** in `e` if *there exists* a free occurrence of `x` in `e`

<br>


We can formally define the set of _all free variables_ in a term like so:

(I) lecture

    ```haskell
    FV(x)       = ???
    FV(\x -> e) = ???
    FV(e1 e2)   = ???
    ```

(I) final

    ```haskell
    FV(x)       = {x}
    FV(\x -> e) = FV(e) \ {x}
    FV(e1 e2)   = FV(e1) + FV(e2)
    ```

<br>
<br>
<br>
<br>
<br>
<br>
<br>
<br>
<br>
<br>
<br>
<br>


## Closed Expressions

If `e` has _no free variables_ it is said to be **closed**

- Closed expressions are also called **combinators**

<br>
<br>

What is the shortest closed expression?

(I) final

    _Answer:_ `\x -> x`

<br>
<br>
<br>
<br>
<br>
<br>
<br>
<br>
<br>
<br>
<br>
<br>

## Rewrite Rules of Lambda Calculus

<br>

1. $\alpha$-step  (aka _renaming formals_)
2. $\beta$-step   (aka _function call_)

<br>
<br>
<br>
<br>
<br>
<br>
<br>
<br>
<br>
<br>
<br>
<br>

## Semantics: $\beta$-Reduction

<br>

```
  (\x -> e1) e2   =b>   e1[x := e2]
```
<br>
where `e1[x := e2]` means
"`e1` with all _free_ occurrences of `x` replaced with `e2`"

<br>
<br>

Computation by _search-and-replace_:

- If you see an _abstraction_ applied to an _argument_,
take the _body_ of the abstraction and
replace all free occurrences of the _formal_ by that _argument_

- We say that `(\x -> e1) e2` $\beta$-steps to `e1[x := e2]`



<br>
<br>
<br>
<br>
<br>
<br>
<br>
<br>
<br>
<br>
<br>
<br>

## Examples

<br>

```haskell
(\x -> x) apple     
=b> apple
```

Is this right? Ask [Elsa](http://goto.ucsd.edu:8095/index.html#?demo=blank.lc)!

<br>
<br>

(I) lecture

    ```haskell
    (\f -> f (\x -> x)) (give apple)
    =b> ???
    ```

(I) final

    ```haskell
    (\f -> f (\x -> x)) (give apple)
    =b> give apple (\x -> x)
    ```

<br>
<br>
<br>
<br>
<br>
<br>
<br>
<br>
<br>
<br>
<br>
<br>

## QUIZ

<br>

```haskell
(\x -> (\y -> y)) apple
=b> ???
```

**A.** `apple`

**B.** `\y -> apple`

**C.** `\x -> apple`

**D.** `\y -> y`

**E.** `\x -> y`


<br>

(I) final

    _Correct answer:_ **D.**

<br>
<br>
<br>
<br>
<br>
<br>
<br>
<br>
<br>
<br>
<br>

## QUIZ

<br>

```haskell
(\x -> x (\x -> x)) apple
=b> ???
```

**A.** `apple (\x -> x)`

**B.** `apple (\apple -> apple)`

**C.** `apple (\x -> apple)`

**D.** `apple`

**E.** `\x -> x`


<br>

(I) final

    _Correct answer:_ **A.**
    
<br>
<br>
<br>
<br>
<br>
<br>
<br>
<br>
<br>
<br>
<br>

## A Tricky One

<br>

```haskell
(\x -> (\y -> x)) y
=b> \y -> y
```

Is this right?

<br>
<br>
<br>
<br>
<br>
<br>
<br>
<br>
<br>
<br>
<br>
<br>

## Something is Fishy

<br>

```haskell
(\x -> (\y -> x)) y
=b> \y -> y
```

Is this right?

**Problem**: the _free_ `y` in the argument has been **captured** by `\y`!

**Solution**: make sure that all _free variables_ of the argument
are different from the binders in the body. 

<br>
<br>
<br>
<br>
<br>
<br>
<br>
<br>
<br>
<br>
<br>
<br>

## Capture-Avoiding Substitution

We have to fix our definition of $\beta$-reduction:

```
  (\x -> e1) e2   =b>   e1[x := e2]
```
<br>
where `e1[x := e2]` means
~~"`e1` with all _free_ occurrences of `x` replaced with `e2`"~~

  - `e1` with all _free_ occurrences of `x` replaced with `e2`,
   **as long as** no free variables of `e2` get captured
  - undefined otherwise

<br>  

Formally:

```haskell
x[x := e]            = e
y[x := e]            = y            -- assuming x /= y
(e1 e2)[x := e]      = (e1[x := e]) (e2[x := e])
(\x -> e1)[x := e]   = \x -> e1     -- why do we leave `e1` alone?
(\y -> e1)[x := e] 
  | not (y in FV(e)) = \y -> e1[x := e]
  | otherise         = undefined    -- wait, but what do we do then???

```

(I) final
    
    *Answer*: We leave `e1` above alone even though it might contain `x`, 
    because in `\x -> e1` every occurrence of `x` is bound by `\x`
    (hence, there are *no free occurrences* of `x`)

<br>
<br>
<br>
<br>
<br>
<br>
<br>
<br>
<br>
<br>
<br>



## Rewrite Rules of Lambda Calculus

<br>

1. $\alpha$-step  (aka _renaming formals_)
2. $\beta$-step   (aka _function call_)

<br>
<br>
<br>
<br>
<br>
<br>
<br>
<br>
<br>
<br>
<br>
<br>

## Semantics: $\alpha$-Renaming

<br>

```haskell
  \x -> e   =a>   \y -> e[x := y]
    where not (y in FV(e))
```
<br>

- We can rename a formal parameter and replace all its occurrences in the body

- We say that `\x -> e` $\alpha$-steps to `\y -> e[x := y]`

<br>
<br>

Example:

```haskell
\x -> x   =a>   \y -> y   =a>    \z -> z
```

All these expressions are **$\alpha$-equivalent**

<br>
<br>
<br>

What's wrong with these?

```haskell
-- (A)
\f -> f x    =a>   \x -> x x
```

(I) final

    *Answer:* it violates the side-condition for $\alpha$-renaming that the new formal (`x`) must not occur freely in the body 

```haskell
-- (B)
(\x -> \y -> y) y   =a>   (\x -> \z -> z) z
```

(I) final
     
    *Answer:* we should only rename within the body of the abstraction; the second `y` is a free variable, and hence must remain unchanged     

```haskell
-- (C)
\x -> \y -> x y   =a>    \apple -> \orange -> apple orange
```
     
(I) final
     
    *Answer:* it's fine, but technically it's two $\alpha$-steps and not one

<br>
<br>
<br>
<br>
<br>
<br>
<br>
<br>
<br>
<br>
<br>
<br>
<br>


## The Tricky One

<br>

(I) lecture

    ```haskell
    (\x -> (\y -> x)) y
    =a> ???
    ```
    
(I) final

    ```haskell
    (\x -> (\y -> x)) y
    =a> (\x -> (\z -> x)) y
    =b> \z -> y
    ```
    
<br>
<br>
To avoid getting confused, you can always rename formals, so that different variables have different names!

<br>
<br>
<br>
<br>
<br>
<br>
<br>
<br>
<br>
<br>
<br>
<br>




## Normal Forms

A **redex** is a $\lambda$-term of the form

`(\x -> e1) e2`

A $\lambda$-term is in **normal form** if it contains no redexes.


<br>
<br>
<br>
<br>
<br>
<br>
<br>
<br>
<br>
<br>
<br>
<br>
<br>

## QUIZ

Which of the following term are **not** in _normal form_ ?

**A.** `x`

**B.** `x y`

**C.** `(\x -> x) y`

**D.** `x (\y -> y)`

**E.** C and D

(I) final
     
    *Answer:* C

<br>
<br>
<br>
<br>
<br>
<br>
<br>
<br>
<br>
<br>
<br>
<br>



## Semantics: Evaluation

A $\lambda$-term `e` **evaluates to** `e'` if

1. There is a sequence of steps
```haskell
e =?> e_1 =?> ... =?> e_N =?> e'
```

   where each `=?>` is either `=a>` or `=b>` 
   and `N >= 0`

2. `e'` is in _normal form_


<br>
<br>
<br>
<br>
<br>
<br>


## Examples of Evaluation

```haskell
(\x -> x) apple
  =b> apple
```

<br> 

(I) lecture
         
    ```haskell
    (\f -> f (\x -> x)) (\x -> x)
      =?> ???
    ```
    
(I) final
         
    ```haskell
    (\f -> f (\x -> x)) (\x -> x)
      =b> (\x -> x) (\x -> x)
      =b> \x -> x
    ```
    
<br>    

(I) lecture
    
    ```haskell
    (\x -> x x) (\x -> x)
      =?> ???
    ```

(I) final
         
    ```haskell
    (\x -> x x) (\x -> x)
      =b> (\x -> x) (\x -> x)
      =b> \x -> x
    ```

<br>
<br>
<br>
<br>
<br>
<br>


## Elsa shortcuts

Named $\lambda$-terms:

```
let ID = \x -> x  -- abbreviation for \x -> x
```

<br>
<br>

To substitute name with its definition, use a `=d>` step:

```haskell
ID apple
  =d> (\x -> x x) apple  -- expand definition
  =b> apple              -- beta-reduce
```

<br>
<br>

Evaluation:

- `e1 =*> e2`: `e1` reduces to `e2` in 0 or more steps
    - where each step is `=a>`, `=b>`, or `=d>`
- `e1 =~> e2`: `e1` evaluates to `e2`

_What is the difference?_


<br>
<br>
<br>
<br>
<br>
<br>
<br>
<br>
<br>
<br>
<br>
<br>

## Non-Terminating Evaluation

```haskell
(\x -> x x) (\x -> x x)
  =b> (\x -> x x) (\x -> x x)
```

Oops, we can write programs that loop back to themselves...

and never reduce to a normal form!

This combinator is called $\Omega$

<br>
<br>
<br>
<br>
<br>
<br>

What if we pass $\Omega$ as an argument to another function?

```
let OMEGA = (\x -> x x) (\x -> x x)

(\x -> \y -> y) OMEGA
```

Does this reduce to a normal form? Try it at home!

<br>
<br>
<br>
<br>
<br>
<br>
<br>
<br>
<br>

## Programming in $\lambda$-calculus

*Real languages have lots of features*

- Booleans
- Records (structs, tuples)
- Numbers
- **Functions** \[we got those\]
- Recursion

Lets see how to _encode_ all of these features
with the $\lambda$-calculus.


<br>
<br>
<br>
<br>
<br>
<br>
<br>
<br>
<br>
<br>
<br>
<br>

## $\lambda$-calculus: Booleans

<br>

How can we encode Boolean values (`TRUE` and `FALSE`) as functions?

<br>

Well, what do we **do** with a Boolean `b`?

<br>
<br>
<br>
<br>
<br>
<br>
<br>
<br>
<br>
<br>
<br>
<br>


Make a *binary choice*

  - `if b then e1 else e2`

<br>
<br>
<br>

## Booleans: API

We need to define three functions

```haskell
let TRUE  = ???
let FALSE = ???
let ITE   = \b x y -> ???  -- if b then x else y
```

such that

```haskell
ITE TRUE apple banana =~> apple
ITE FALSE apple banana =~> banana
```

(Here, `let NAME = e` means `NAME` is an _abbreviation_ for `e`)


<br>
<br>
<br>
<br>
<br>
<br>
<br>
<br>
<br>
<br>
<br>
<br>

## Booleans: Implementation

```haskell
let TRUE  = \x y -> x        -- Returns its first argument
let FALSE = \x y -> y        -- Returns its second argument
let ITE   = \b x y -> b x y  -- Applies condition to branches
                             -- (redundant, but improves readability)
```

<br>
<br>
<br>
<br>
<br>
<br>
<br>
<br>
<br>
<br>
<br>
<br>



## Example: Branches step-by-step


```haskell
eval ite_true:
  ITE TRUE e1 e2
  =d> (\b x y -> b    x  y) TRUE e1 e2    -- expand def ITE  
  =b>   (\x y -> TRUE x  y)      e1 e2    -- beta-step
  =b>     (\y -> TRUE e1 y)         e2    -- beta-step
  =b>            TRUE e1 e2               -- expand def TRUE
  =d>     (\x y -> x) e1 e2               -- beta-step
  =b>       (\y -> e1)   e2               -- beta-step
  =b> e1
```


<br>
<br>
<br>
<br>
<br>
<br>

## Example: Branches step-by-step

Now you try it!


Can you [fill in the blanks to make it happen?][elsa-ite]


(I) lecture

    ```haskell
    eval ite_false:
      ITE FALSE e1 e2

      -- fill the steps in!

      =b> e2  
    ```

(I) final

    ```haskell
    eval ite_false:
      ITE FALSE e1 e2
      =d> (\b x y -> b     x  y) FALSE e1 e2   -- expand def ITE  
      =b>   (\x y -> FALSE x  y)       e1 e2   -- beta-step
      =b>     (\y -> FALSE e1 y)          e2   -- beta-step
      =b>            FALSE e1 e2               -- expand def FALSE
      =d>      (\x y -> y) e1 e2               -- beta-step
      =b>        (\y -> y)    e2               -- beta-step
      =b> e2
    ```


<br>
<br>
<br>
<br>
<br>
<br>
<br>
<br>
<br>
<br>
<br>
<br>




## Boolean Operators


Now that we have `ITE` it's easy to define other Boolean operators:


```haskell
let NOT = \b     -> ???

let AND = \b1 b2 -> ???

let OR  = \b1 b2 -> ???
```

<br>
<br>
<br>
<br>
<br>
<br>
<br>
<br>
<br>
<br>
<br>
<br>
<br>
<br>
<br>
<br>
<br>


```haskell
let NOT = \b     -> ITE b FALSE TRUE 

let AND = \b1 b2 -> ITE b1 b2 FALSE

let OR  = \b1 b2 -> ITE b1 TRUE b2
```

<br>
<br>

Or, since `ITE` is redundant:

```haskell
let NOT = \b     -> b FALSE TRUE 

let AND = \b1 b2 -> b1 b2 FALSE

let OR  = \b1 b2 -> b1 TRUE b2
```

<br>

*Which definition to do you prefer and why?*

<br>
<br>
<br>
<br>
<br>
<br>
<br>
<br>
<br>
<br>
<br>

## Programming in $\lambda$-calculus

- **Booleans** \[done\]
- Records (structs, tuples)
- Numbers
- **Functions** \[we got those\]
- Recursion

<br>
<br>
<br>
<br>
<br>
<br>
<br>
<br>
<br>
<br>
<br>
<br>

## $\lambda$-calculus: Records

Let's start with records with _two_ fields (aka **pairs**)

What do we *do* with a pair?

1. **Pack two** items into a pair, then
2. **Get first** item, or
3. **Get second** item.


<br>
<br>
<br>
<br>
<br>
<br>
<br>
<br>
<br>
<br>
<br>
<br>
<br>
<br>

## Pairs : API

We need to define three functions

```haskell
let PAIR = \x y -> ???    -- Make a pair with elements x and y 
                          -- { fst : x, snd : y }
let FST  = \p -> ???      -- Return first element 
                          -- p.fst
let SND  = \p -> ???      -- Return second element
                          -- p.snd
```

such that

```haskell
FST (PAIR apple banana) =~> apple
SND (PAIR apple banana) =~> banana
```


<br>
<br>
<br>
<br>
<br>
<br>
<br>
<br>
<br>
<br>
<br>
<br>


## Pairs: Implementation

A pair of `x` and `y` is just something that lets you pick between `x` and `y`!
(I.e. a function that takes a boolean and returns either `x` or `y`)  

```haskell
let PAIR = \x y -> (\b -> ITE b x y)
let FST  = \p -> p TRUE   -- call w/ TRUE, get first value
let SND  = \p -> p FALSE  -- call w/ FALSE, get second value
```


<br>
<br>
<br>
<br>
<br>
<br>
<br>
<br>
<br>
<br>
<br>
<br>


## Exercise: Triples?

How can we implement a record that contains **three** values?

(I) lecture

    ```haskell
    let TRIPLE = \x y z -> ???
    let FST3  = \t -> ???
    let SND3  = \t -> ???
    let TRD3  = \t -> ???
    ```

(I) final

    ```haskell
    let TRIPLE = \x y z -> PAIR x (PAIR y z)
    let FST3  = \t -> FST t
    let SND3  = \t -> FST (SND t)
    let TRD3  = \t -> SND (SND t)
    ```


<br>
<br>
<br>
<br>
<br>
<br>
<br>
<br>
<br>
<br>
<br>
<br>

## Programming in $\lambda$-calculus

- **Booleans** \[done\]
- **Records** (structs, tuples) \[done\]
- Numbers
- **Functions** \[we got those\]
- Recursion

<br>
<br>
<br>
<br>
<br>
<br>
<br>
<br>
<br>
<br>
<br>
<br>

## $\lambda$-calculus: Numbers

Let's start with **natural numbers** (0, 1, 2, ...)

What do we *do* with natural numbers?

- Count: `0`, `inc`
- Arithmetic: `dec`, `+`, `-`, `*`
- Comparisons: `==`, `<=`, etc

<br>
<br>
<br>
<br>
<br>
<br>
<br>
<br>
<br>
<br>
<br>
<br>

## Natural Numbers: API

We need to define:

- A family of **numerals**: `ZERO`, `ONE`, `TWO`, `THREE`, ...
- Arithmetic functions: `INC`, `DEC`, `ADD`, `SUB`, `MULT`
- Comparisons: `IS_ZERO`, `EQ`

Such that they respect all regular laws of arithmetic, e.g.

```haskell
IS_ZERO ZERO       =~> TRUE
IS_ZERO (INC ZERO) =~> FALSE
INC ONE            =~> TWO
...
```

<br>
<br>
<br>
<br>
<br>
<br>
<br>
<br>
<br>
<br>
<br>
<br>

## Natural Numbers: Implementation

**Church numerals**: _a number `N`_
is encoded as a combinator that
_calls a function on an argument `N` times_

```haskell
let ONE   = \f x -> f x
let TWO   = \f x -> f (f x)
let THREE = \f x -> f (f (f x))
let FOUR  = \f x -> f (f (f (f x)))
let FIVE  = \f x -> f (f (f (f (f x))))
let SIX   = \f x -> f (f (f (f (f (f x)))))
...
```


<br>
<br>
<br>
<br>
<br>
<br>
<br>
<br>
<br>
<br>
<br>
<br>

## QUIZ: Church Numerals

Which of these is a valid encoding of `ZERO` ?

- **A**: `let ZERO = \f x -> x`

- **B**: `let ZERO = \f x -> f`

- **C**: `let ZERO = \f x -> f x`

- **D**: `let ZERO = \x -> x`

- **E**: None of the above

(I) final

    *Answer:* A

<br>
<br>
<br>

Does this function look familiar?

(I) final

    *Answer:* It's the same as `FALSE`!

<br>
<br>
<br>
<br>
<br>
<br>
<br>
<br>
<br>
<br>
<br>


## $\lambda$-calculus: Increment

(I) lecture

    ```haskell
    -- Call `f` on `x` one more time than `n` does
    let INC   = \n -> (\f x -> ???)
    ```
    
(I) final

    ```haskell
    -- Call `f` on `x` one more time than `n` does
    let INC   = \n -> (\f x -> f (n f x))
    ```
    

<br>
<br>
<br>
<br>
<br>
<br>
<br>
<br>
<br>
<br>
<br>
<br>

**Example:**

```haskell
eval inc_zero :
  INC ZERO
  =d> (\n f x -> f (n f x)) ZERO
  =b> \f x -> f (ZERO f x)
  =*> \f x -> f x
  =d> ONE
```

<br>
<br>
<br>
<br>
<br>
<br>
<br>
<br>
<br>
<br>
<br>
<br>

## QUIZ

How shall we implement `ADD`?


**A.**  `let ADD = \n m -> n INC m`

**B.**  `let ADD = \n m -> INC n m`

**C.**  `let ADD = \n m -> n m INC`

**D.**  `let ADD = \n m -> n (m INC)`

**E.**  `let ADD = \n m -> n (INC m)`

(I) final

    *Answer:* A


<br>
<br>
<br>
<br>
<br>
<br>
<br>
<br>
<br>
<br>
<br>
<br>

$\lambda$-calculus: Addition


```haskell
--  Call `f` on `x` exactly `n + m` times
let ADD = \n m -> n INC m
```

<br>
<br>
<br>

**Example:**

```haskell
eval add_one_zero :
  ADD ONE ZERO
  =~> ONE
```

<br>
<br>
<br>
<br>
<br>
<br>
<br>
<br>
<br>
<br>
<br>
<br>


## QUIZ

How shall we implement `MULT`?

**A.**  `let MULT = \n m -> n ADD m`

**B.**  `let MULT = \n m -> n (ADD m) ZERO`

**C.**  `let MULT = \n m -> m (ADD n) ZERO`

**D.**  `let MULT = \n m -> n (ADD m ZERO)`

**E.**  `let MULT = \n m -> (n ADD m) ZERO`

(I) final

    *Answer:* B or C

<br>
<br>
<br>
<br>
<br>
<br>
<br>
<br>
<br>
<br>
<br>
<br>

## $\lambda$-calculus: Multiplication

```haskell
--  Call `f` on `x` exactly `n * m` times
let MULT = \n m -> n (ADD m) ZERO
```

<br>
<br>
<br>

**Example:**

```haskell
eval two_times_three :
  MULT TWO ONE
  =~> TWO
```

<br>
<br>
<br>
<br>
<br>
<br>
<br>
<br>
<br>
<br>
<br>
<br>

## Programming in $\lambda$-calculus

- **Booleans** \[done\]
- **Records** (structs, tuples) \[done\]
- **Numbers** \[done\]
- **Functions** \[we got those\]
- Recursion

<br>
<br>
<br>
<br>
<br>
<br>
<br>
<br>
<br>
<br>
<br>
<br>

## $\lambda$-calculus: Recursion

<br>

I want to write a function that sums up natural numbers up to `n`:

```
\n -> ...          -- 1 + 2 + ... + n
```

<br>
<br>
<br>
<br>
<br>
<br>
<br>
<br>
<br>
<br>

## QUIZ

Is this a correct implementation of `SUM`?

```
let SUM = \n -> ITE (ISZ n) 
            ZERO 
            (ADD n (SUM (DEC n)))
```

**A.**  Yes

**B.**  No

<br>
<br>
<br>
<br>
<br>
<br>
<br>
<br>
<br>
<br>

No! 

  * Named terms in Elsa are just syntactic sugar
  * To translate an Elsa term to $\lambda$-calculus: replace each name with its definition

```
\n -> ITE (ISZ n) 
        ZERO 
        (ADD n (SUM (DEC n))) -- But SUM is not a thing!
```

<br>
<br>

**Recursion:** 

 - Inside this function I want to call *the same function* on `DEC n`

<br>
<br>

Looks like we can't do recursion,
because it requires being able to refer to functions *by name*,
but in $\lambda$-calculus functions are *anonymous*.

Right?

<br>
<br>
<br>
<br>
<br>
<br>
<br>
<br>
<br>
<br>
<br>
<br>

## $\lambda$-calculus: Recursion

Think again!

<br>
<br>

**Recursion:** 

 - ~~Inside this function I want to call *the same function* on `DEC n`~~
 - Inside this function I want to call *a function* on `DEC n`
 - *And BTW,* I want it to be the same function 
 
<br>
<br>

**Step 1:** Pass in the function to call "recursively"
 
```
let STEP = 
  \rec -> \n -> ITE (ISZ n) 
                  ZERO 
                  (ADD n (rec (DEC n))) -- Call some rec
```
<br>
<br>

**Step 2:** Do something clever to `STEP`, so that the function passed as `rec`
itself becomes

```
\n -> ITE (ISZ n) ZERO (ADD n (rec (DEC n)))
```
 
<br>
<br>
<br>
<br>
<br>
<br>
<br>
<br>
<br>
<br>
<br>
<br>
 
## $\lambda$-calculus: Fixpoint Combinator 

**Wanted:** a combinator `FIX` such that `FIX STEP`
calls `STEP` with itself as the first argument:

```
FIX STEP
=*> STEP (FIX STEP)
```

<br>

(In math: a *fixpoint* of a function $f(x)$ is a point $x$, such that $f(x) = x$)

<br>
<br>
<br>
<br>

Once we have it, we can define:

```
let SUM = FIX STEP
```

Then by property of `FIX` we have:
```
SUM =*> STEP SUM -- (1)
```


```
eval sum_one:
  SUM ONE
  =*> STEP SUM ONE                 -- (1)
  =d> (\rec n -> ITE (ISZ n) ZERO (ADD n (rec (DEC n)))) SUM ONE
  =b> (\n -> ITE (ISZ n) ZERO (ADD n (SUM (DEC n)))) ONE 
                                   -- ^^^ the magic happened!
  =b> ITE (ISZ ONE) ZERO (ADD ONE (SUM (DEC ONE)))
  =*> ADD ONE (SUM ZERO)           -- def of ISZ, ITE, DEC, ...
  =*> ADD ONE (STEP SUM ZERO)      -- (1)
  =d> ADD ONE 
        ((\rec n -> ITE (ISZ n) ZERO (ADD n (rec (DEC n)))) SUM ZERO)
  =b> ADD ONE ((\n -> ITE (ISZ n) ZERO (ADD n (SUM (DEC n)))) ZERO)
  =b> ADD ONE (ITE (ISZ ZERO) ZERO (ADD ZERO (SUM (DEC ZERO))))
  =b> ADD ONE ZERO
  =~> ONE
```


How should we define `FIX`???

<br>
<br>
<br>
<br>
<br>
<br>
<br>
<br>
<br>
<br>
<br>
<br>

## The Y combinator 
 
Remember $\Omega$?
 
```haskell
(\x -> x x) (\x -> x x)
=b> (\x -> x x) (\x -> x x)
``` 
 
This is *self-replcating code*! We need something like this but a bit more involved...

<br>
<br>
<br>
<br>

The Y combinator discovered by Haskell Curry:

```haskell
let FIX   = \stp -> (\x -> stp (x x)) (\x -> stp (x x))
``` 
<br>
<br>

How does it work?

```haskell
eval fix_step:
  FIX STEP
  =d> (\stp -> (\x -> stp (x x)) (\x -> stp (x x))) STEP
  =b> (\x -> STEP (x x)) (\x -> STEP (x x))
  =b> STEP ((\x -> STEP (x x)) (\x -> STEP (x x)))
  --       ^^^^^^^^^^ this is FIX STEP ^^^^^^^^^^^
``` 

<br>
<br>
<br>
<br>
<br>

That's all folks!


[elsa-ite]: http://goto.ucsd.edu:8095/index.html#?demo=ite.lc

[elsa-not]: http://goto.ucsd.edu:8095/index.html#?demo=permalink%2F1491005489_149.lc
